lib/Buckets/PackedKVMarshalling.i.dfy
@@ -1,0 +1,113 @@
+include "../Base/Option.s.dfy"
+include "../Marshalling/GenericMarshalling.i.dfy"
+include "PackedStringArrayMarshalling.i.dfy"
+include "PackedKV.i.dfy"
+include "BucketWeights.i.dfy"
+
+module PackedKVMarshalling {
+  import opened Options
+  import PSA = PackedStringArray
+  import opened GenericMarshalling
+  import opened NativeTypes
+  import PSAMarshalling = PackedStringArrayMarshalling
+  import opened PackedKV
+  import opened ValueMessage
+  import BW = BucketWeights
+  
+  function method grammar() : G
+    ensures ValidGrammar(grammar())
+  {
+    GTuple([
+      PSAMarshalling.grammar(), // keys
+      PSAMarshalling.grammar()  // messages
+    ])
+  }
+
+  function fromVal(v: V) : (opkv: Option<Pkv>)
+    requires ValInGrammar(v, grammar())
+    ensures opkv.Some? ==> WF(opkv.value)
+  {
+    var okeys := PSAMarshalling.fromVal(v.t[0]);
+    var omsgs := PSAMarshalling.fromVal(v.t[1]);
+    if okeys.Some? && omsgs.Some? then (
+      var pkv := Pkv(okeys.value, omsgs.value);
+      if WF(pkv) then
+        Some(pkv)
+      else
+        None
+    ) else
+      None
+  }
+
+  function toVal(pkv: Pkv) : (v: V)
+    requires WF(pkv)
+    ensures ValInGrammar(v, grammar())
+  {
+    VTuple([PSAMarshalling.toVal(pkv.keys), PSAMarshalling.toVal(pkv.messages)])
+  }
+
+  lemma parseMarshalledCorrect(pkv: Pkv)
+    requires WF(pkv)
+    ensures fromVal(toVal(pkv)) == Some(pkv)
+  {
+  }
+
+  // lemma SizeOfV_WeightBucket(pkv: Pkv)
+  //   requires WF(pkv)
+  //   requires Keyspace.IsStrictlySorted(PSA.I(pkv.keys))
+  //   ensures SizeOfV(toVal(pkv)) == 16 + BW.WeightBucket(I(pkv))
+  // {
+  //   assume false;
+  // }
+  
+  method ComputeWF(pkv: Pkv) returns (result: bool)
+    requires PSA.WF(pkv.keys)
+    requires PSA.WF(pkv.messages)
+    ensures result == WF(pkv)
+  {
+    var vkl := ComputeValidStringLens(pkv.keys, KeyType.MaxLen());
+    var vml := ComputeValidStringLens(pkv.messages, ValueType.MaxLen());
+    assume IdentityMessage() !in IMessages(pkv.messages); // FIXME(robj): can we eliminate this from WF()?
+    result :=
+      && PSA.psaNumStrings(pkv.keys) == PSA.psaNumStrings(pkv.messages)
+      && vkl
+      && vml;
+    if result {
+      assert WF(pkv);
+    } else {
+      assert !WF(pkv);
+    }
+  }
+  
+  method FromVal(v: V) returns (pkv: Option<Pkv>)
+    requires ValInGrammar(v, grammar())
+    requires ValidVal(v)
+    ensures pkv == fromVal(v)
+  {
+    var okeys := PSAMarshalling.FromVal(v.t[0]);
+    var omessages := PSAMarshalling.FromVal(v.t[1]);
+    if okeys.Some? && omessages.Some? {
+      var tmp := Pkv(okeys.value, omessages.value);
+      var wf := ComputeWF(tmp);
+      if wf {
+        pkv := Some(tmp);
+      } else {
+        pkv := None;
+      }
+    } else {
+      pkv := None;
+    }
+  }
+
+  method ToVal(pkv: Pkv) returns (v: V)
+    requires WF(pkv)
+    ensures ValInGrammar(v, grammar())
+    ensures v == toVal(pkv)
+    ensures ValidVal(v)
+  {
+    var vkeys := PSAMarshalling.ToVal(pkv.keys);
+    var vmessages := PSAMarshalling.ToVal(pkv.messages);
+    v := VTuple([vkeys, vmessages]);
+  }
+
+}
